faster MuRec extraction

theories/L/Reductions/MuRec/MuRec_extract.v
@@ -12,44 +12,53 @@ Inductive reccode :=
 | rc_rec (f : reccode) (g : reccode)
 | rc_min (f : reccode).
 
+Definition id_Some_inl (o : option (nat + list nat)) : option (nat + list nat) :=
+  match o with
+  | Some (inl f) => o
+  | _ => None
+  end.
+
+#[global] Arguments id_Some_inl /.
+
+Definition eval_rec (eval : nat -> reccode -> list nat -> option (nat + list nat)) (min : nat) (c : reccode) (v : list nat) : option (nat + list nat) :=
+  match c with
+  | rc_cst n => Some (inl n)
+  | rc_zero => Some (inl 0)
+  | rc_succ => match v with
+              | x :: _ => Some (inl (S x))
+              | _ => None
+              end
+  | rc_proj n => option_map inl (nth_error v n)
+  | rc_comp f g => match eval min g v
+                  with
+                  | Some (inr g) => id_Some_inl (eval min f g)
+                  | _ => None
+                  end
+  | rc_cons f g => match eval min f v, eval min g v with
+                  | Some (inl f), Some (inr g) => Some (inr (f :: g))
+                  | _, _ => None
+                  end
+  | rc_nil => Some (inr nil)
+  | rc_rec f g => match v with
+                  | 0 :: v => id_Some_inl (eval min f v)
+                  | S n :: v => match eval min (rc_rec f g) (n :: v) with
+                              | Some (inl y) => id_Some_inl (eval min g (n :: y :: v))
+                              | _ => None
+                              end
+                  | _ => None
+                  end
+  | rc_min f => match eval 0 f (min :: v) with
+                | Some (inl 0) => Some (inl min)
+                | Some (inl _) => id_Some_inl (eval (S min) (rc_min f) v)
+                | _ => None
+                end
+  end.
+
 Fixpoint eval (fuel : nat) (min : nat) (c : reccode) (v : list nat) : option (nat + list nat) :=
   match fuel with
   | 0 => None
-  | S fuel =>
-    match c with
-    | rc_cst n => Some (inl n)
-    | rc_zero => Some (inl 0)
-    | rc_succ => match v with
-                | x :: _ => Some (inl (S x))
-                | _ => None
-                end
-    | rc_proj n => match nth_error v n with Some r => Some (inl r) | None => None end
-    | rc_comp f g => match eval fuel min g v
-                    with
-                    | Some (inr g) => match eval fuel min f g with Some (inl f) => Some (inl f) | _ => None end
-                    | _ => None
-                    end
-    | rc_cons f g => match eval fuel min f v, eval fuel min g v with
-                    | Some (inl f), Some (inr g) => Some (inr (f :: g))
-                    | _, _ => None
-                    end
-    | rc_nil => Some (inr nil)
-    | rc_rec f g => match v with
-                   | 0 :: v => match eval fuel min f v with Some (inl r) => Some (inl r) | _ => None end
-                   | S n :: v => match eval fuel min (rc_rec f g) (n :: v) with
-                               | Some (inl y) => match eval fuel min g (n :: y :: v) with Some (inl r) => Some (inl r) | _ => None end
-                               | _ => None
-                               end
-                   | _ => None
-                   end
-    | rc_min f => match eval fuel 0 f (min :: v) with
-                 | Some (inl 0) => Some (inl min)
-                 | Some (inl _) => match eval fuel (S min) (rc_min f) v with Some (inl r) => Some (inl r) | _ => None end
-                 | _ => None
-                 end
-    end
+  | S fuel => eval_rec (eval fuel) min c v
   end.
-
 
 MetaCoq Run (tmGenEncode "enc_reccode" reccode).
 #[export] Hint Resolve enc_reccode_correct : Lrewrite.
@@ -62,8 +71,11 @@ Instance term_rc_cons : computable rc_cons. Proof. extract constructor. Qed.
 Instance term_rc_rec : computable rc_rec. Proof. extract constructor. Qed.
 #[global]
 Instance term_rc_min : computable rc_min. Proof. extract constructor. Qed.
-#[global]
-Instance term_eval : computable eval.
+#[local] Instance term_id_Some_inl : computable id_Some_inl.
+Proof. extract. Qed.
+#[local] Instance term_eval_rec : computable eval_rec.
+Proof. extract. Qed.
+#[global] Instance term_eval : computable eval.
 Proof.
   extract.
 Qed.
